---
title: "4-1"
author: "Kai"
date: "23 Dezember 2016"
output: pdf_document
---

$$
\begin{aligned}
s^2 &= \underbrace{(y-X\beta)'(y-X\hat{\beta})}_{SSE} / (n-K-1)
\end{aligned}
$$

$$
\begin{aligned}
SEE &= y'(I-X(X'X)^{-1}X')y\\
E(SEE) &= (tr(I-X(X'X)^{-1}X')\sigma^2 V)+E(y')(I-X(X'X)^{-1}X')E(y)\\
&= \sigma^2 tr(V-X(X'X)^{-1}X'V)+\underbrace{\beta'X'(I-X(X'X)^{-1}X')X\beta}_{=0}\\
&= \sigma^2(tr(V)-tr(X(X'X)^{-1}X'V))\\
&= \sigma^2(tr((1-\rho)I_n+\rho 1_n 1_n')-tr(X(X'X)^{-1}X'((1-\rho)I_n+\rho 1_n 1_n')))\\
&=\sigma^2((1-\rho)n+\rho n - (1-\rho)(K+1)+ \underbrace{\rho tr(X(X'X)^{-1}X'-1_n1_n')}_{non-singular})\\
&=\sigma^2((1-\rho)n+\rho n - (1-\rho)(K+1)+ \rho tr(X(X'X)^{-1}X'X(X'X)^{-1}-I))\\
&=\sigma^2((1-\rho)n+\rho n - (1-\rho)(K+1)+ \rho tr(HH^{-1}I))\\
&=\sigma^2((1-\rho)n+\rho n - (1-\rho)(K+1)+ \rho tr(I))\\
&=\sigma^2((1-\rho)n+\rho n - (1-\rho)(K+1)+ \rho n\\
\end{aligned}
$$

$$
\begin{aligned}
E(s^2) &= \frac{\sigma^2(n-K-1)(1-\rho)}{n-K-1}\\
&= \sigma^2(1-\rho)
\end{aligned}
$$

$$
\begin{aligned}
Cov(y) &= \sigma^2V; V = (1-\rho)I_n+\rho 1_n 1_n'
\end{aligned}
$$

The covariance structure implies the same positive correlation $\rho$ between any two observations and the same variance for all observations.